proof/proof/auditor_proof/rpc_serv.v
@@ -1,0 +1,311 @@
+From New.generatedproof.github_com.sanjit_bhat.pav Require Import auditor server.
+From New.proof.github_com.sanjit_bhat.pav Require Import prelude.
+
+From New.proof.github_com.sanjit_bhat.pav Require Import
+  advrpc cryptoffi hashchain ktcore merkle.
+
+From New.proof.github_com.sanjit_bhat.pav.auditor_proof Require Import
+  serde.
+From New.proof.github_com.sanjit_bhat.pav.server_proof Require Import
+  serde server rpc.
+
+Module auditor.
+Import serde.server server.server rpc.server serde.auditor.
+
+Module state.
+Record t :=
+  mk {
+    digs: list $ list w8;
+  }.
+End state.
+
+(* cfg is the static state we know about this party, if good. *)
+Module cfg.
+Record t :=
+  mk {
+    (* duplicate [serv_sig_pk] across [serv_good] bc we need to know
+    it unconditionally. *)
+    serv_sig_pk: list w8;
+    adtr_sig_pk: list w8;
+    agreeγ: ktcore.Agree.t;
+    serv_good: server.Trust.t;
+  }.
+End cfg.
+
+Section proof.
+Context `{!heapGS Σ}.
+Context {sem : go.Semantics}.
+Collection W := sem.
+#[local] Set Default Proof Using "W".
+
+Definition wish_SignedLink servPk adtrPk ep link : iProp Σ :=
+  "#Hwish_adtr_sig" ∷ ktcore.wish_LinkSig adtrPk ep
+    link.(SignedLink.Link) link.(SignedLink.AdtrSig) ∗
+  "#Hwish_serv_sig" ∷ ktcore.wish_LinkSig servPk ep
+    link.(SignedLink.Link) link.(SignedLink.ServSig).
+
+Definition wish_SignedVrf servPk adtrPk vrf : iProp Σ :=
+  "#Hwish_adtr_sig" ∷ ktcore.wish_VrfSig adtrPk
+    vrf.(SignedVrf.VrfPk) vrf.(SignedVrf.AdtrSig) ∗
+  "#Hwish_serv_sig" ∷ ktcore.wish_VrfSig servPk
+    vrf.(SignedVrf.VrfPk) vrf.(SignedVrf.ServSig).
+
+End proof.
+
+Module history.
+Section proof.
+Context `{!heapGS Σ}.
+Context {sem : go.Semantics}.
+Collection W := sem.
+#[local] Set Default Proof Using "W".
+
+Definition own_ep ptr σ (ep : nat) γ : iProp Σ :=
+  let agreeγ := γ.(cfg.agreeγ) in
+  ∃ sig_link,
+  "#Hown_epoch" ∷ SignedLink.own ptr sig_link (□) ∗
+  "#His_epoch" ∷ wish_SignedLink γ.(cfg.serv_sig_pk) γ.(cfg.adtr_sig_pk)
+    (W64 ep) sig_link ∗
+  (* could derive this from LinkSig, but it's easier to state explicitly. *)
+  "%His_link" ∷ ⌜hashchain.valid (take (S ep - agreeγ.(ktcore.Agree.digs_start)) σ.(state.digs))
+    agreeγ.(ktcore.Agree.cut) sig_link.(SignedLink.Link) (S ep)⌝.
+
+(* TODO: in-mem startEp and sigpred startEp are diff values.
+we should give them diff names. *)
+Definition own ptr γ σ q : iProp Σ :=
+  let agreeγ := γ.(cfg.agreeγ) in
+  ∃ sl_lastDig lastDig start_ep sl_epochs sl0_epochs,
+  let last_ep := agreeγ.(ktcore.Agree.digs_start) + length σ.(state.digs) - 1 in
+  "Hstr_history" ∷ ptr ↦{#q} (auditor.history.mk sl_lastDig start_ep sl_epochs) ∗
+  "#Hsl_lastDig" ∷ sl_lastDig ↦*□ lastDig ∗
+  "%Heq_lastDig" ∷ ⌜last σ.(state.digs) = Some lastDig⌝ ∗
+  "Hsl_epochs" ∷ sl_epochs ↦*{#q} sl0_epochs ∗
+  "Hcap_epochs" ∷ own_slice_cap loc sl_epochs (DfracOwn q) ∗
+  "#Hepochs" ∷ ([∗ list] idx ↦ ptr ∈ sl0_epochs,
+    own_ep ptr σ (uint.nat start_ep + idx)%nat γ) ∗
+
+  "%Hsome_digs" ∷ ⌜length σ.(state.digs) > 0⌝ ∗
+  "%Hsome_epochs" ∷ ⌜length sl0_epochs > 0⌝ ∗
+  "%Hnoof_ep" ∷ ⌜last_ep = uint.Z $ W64 last_ep⌝ ∗
+  "%Heq_audit_start" ∷ ⌜uint.nat start_ep = (agreeγ.(ktcore.Agree.digs_start) + agreeγ.(ktcore.Agree.func_start))%nat⌝ ∗
+  "%Heq_audit_end" ∷ ⌜(uint.nat start_ep + length sl0_epochs =
+    agreeγ.(ktcore.Agree.digs_start) + length σ.(state.digs))%nat⌝.
+
+Definition align_serv σ γ servγ : iProp Σ :=
+  let agreeγ := γ.(cfg.agreeγ) in
+  let servAgreeγ := servγ.(server.cfg.agreeγ) in
+  ∃ digs,
+  "#His_digs" ∷ mono_list_lb_own servAgreeγ.(ktcore.Agree.digs) digs ∗
+  "%Heq_digs" ∷ ⌜σ.(state.digs) = digs⌝ ∗
+  "%Heq_digs_start" ∷ ⌜agreeγ.(ktcore.Agree.digs_start) = 0%nat⌝ ∗
+  "%Heq_cut" ∷ ⌜agreeγ.(ktcore.Agree.cut) = None⌝.
+
+#[global] Instance own_aux_combine_sep_as ptr γ σ0 σ1 q0 q1 :
+  CombineSepAs (own ptr γ σ0 q0) (own ptr γ σ1 q1) (own ptr γ σ0 (q0 + q1)) | 60.
+Proof.
+  rewrite /CombineSepAs.
+  iIntros "[H0 H1]".
+  iNamedSuffix "H0" "0".
+  iNamedSuffix "H1" "1".
+  iCombine "Hstr_history0 Hstr_history1" as "?" gives %?.
+  simplify_eq/=.
+  iCombine "Hsl_epochs0 Hsl_epochs1" as "?" gives %?.
+  iCombine "Hcap_epochs0 Hcap_epochs1" as "?".
+  iCombine "Hsl_lastDig0 Hsl_lastDig1" gives %?.
+  simplify_eq/=.
+  (* TODO: DfracOwn q0 ⋅ DfracOwn q1. not getting combined properly. *)
+  iFrame "∗#%".
+Qed.
+
+#[global] Instance own_frac ptr γ σ :
+  fractional.Fractional (λ q, own ptr γ σ q).
+Proof.
+  intros ??. iSplit.
+  - iIntros "@".
+    iDestruct "Hstr_history" as "[? ?]".
+    iDestruct "Hsl_epochs" as "[? ?]".
+    iDestruct "Hcap_epochs" as "[? ?]".
+    iFrame "∗#%".
+  - iIntros "[H0 H1]".
+    by iCombine "H0 H1" as "H".
+Qed.
+
+#[global] Instance own_as_frac ptr γ σ q :
+  fractional.AsFractional (own ptr γ σ q) (λ q, own ptr γ σ q) q.
+Proof. auto. Qed.
+
+End proof.
+End history.
+
+Section proof.
+Context `{!heapGS Σ}.
+Context {sem : go.Semantics} {package_sem : auditor.Assumptions}.
+Collection W := sem + package_sem.
+#[local] Set Default Proof Using "W".
+
+Definition wish_getNextLink γ σ proof (ep : w64) dig link : iProp Σ :=
+  let agreeγ := γ.(cfg.agreeγ) in
+  ∃ prevDig,
+  "%Heq_ep" ∷ ⌜uint.Z ep = (agreeγ.(ktcore.Agree.digs_start) + length σ.(state.digs))%Z⌝ ∗
+  "%Heq_prevDig" ∷ ⌜last σ.(state.digs) = Some prevDig⌝ ∗
+  "#His_upd" ∷ ktcore.wish_ListUpdate prevDig
+    proof.(ktcore.AuditProof.Updates) dig ∗
+  "%His_link" ∷ ⌜hashchain.valid (σ.(state.digs) ++ [dig]) agreeγ.(ktcore.Agree.cut)
+    link (S $ uint.nat ep)⌝ ∗
+  "#His_sig" ∷ ktcore.wish_LinkSig γ.(cfg.serv_sig_pk) ep link
+    proof.(ktcore.AuditProof.LinkSig).
+
+Lemma wish_getNextLink_det γ σ proof ep0 dig0 link0 ep1 dig1 link1 :
+  wish_getNextLink γ σ proof ep0 dig0 link0 -∗
+  wish_getNextLink γ σ proof ep1 dig1 link1 -∗
+  ⌜ep0 = ep1 ∧ dig0 = dig1 ∧ link0 = link1⌝.
+Proof.
+  iNamedSuffix 1 "0".
+  iNamedSuffix 1 "1".
+  simplify_eq/=.
+  iDestruct (ktcore.wish_ListUpdate_det with "His_upd0 His_upd1") as %->.
+  destruct His_link0 as [His_link0 _].
+  destruct His_link1 as [His_link1 _].
+  rewrite -His_link1 in His_link0.
+  opose proof (hashchain.det _ _ _ _ His_link0) as ->.
+  iPureIntro. repeat split. word.
+Qed.
+
+Lemma wp_CallAudit c good (prevEpoch : w64) :
+  {{{
+    is_pkg_init server ∗
+    "#His_serv" ∷ is_rpc_cli c good ∗
+    "#His_args" ∷ match Trust.get_full good with None => True | Some γ =>
+      let servAgreeγ := γ.(server.cfg.agreeγ) in
+      ∃ entry : list w8,
+      "#Hidx_ep" ∷ mono_list_idx_own servAgreeγ.(ktcore.Agree.digs) (uint.nat prevEpoch) entry end
+  }}}
+  @! server.CallAudit #c #prevEpoch
+  {{{
+    sl_proofs err, RET (#sl_proofs, #(ktcore.blame_to_u64 err));
+    "%Hblame" ∷ ⌜ktcore.BlameSpec err {[ktcore.BlameServFull:=option_bool $ Trust.get_full good]}⌝ ∗
+    "#Herr" ∷ (if decide (err ≠ ∅) then True else
+      ∃ proofs,
+      "#Hsl_proofs" ∷ ktcore.AuditProofSlice1D.own sl_proofs proofs (□) ∗
+
+      "Hgood" ∷ match Trust.get_full good with None => True | Some γ =>
+        (* writing determ trans per epoch makes postcond easier to use
+        than one trans across all epochs. epochs are indep. *)
+        ([∗ list] idx ↦ proof ∈ proofs,
+          □ ∀ agreeγ adtrσ,
+          history.align_serv adtrσ agreeγ γ -∗
+          ⌜length adtrσ.(state.digs) - 1 = (uint.Z prevEpoch + idx)%Z⌝ -∗
+          ⌜agreeγ.(cfg.serv_sig_pk) = γ.(cfg.sig_pk)⌝ -∗
+
+          ∃ ep dig link,
+          let adtrσ' := set state.digs (.++ [dig]) adtrσ in
+          "#Hwish_getNextLink" ∷ wish_getNextLink agreeγ adtrσ
+            proof ep dig link ∗
+          "#Halign_next" ∷ history.align_serv adtrσ' agreeγ γ) end)
+  }}}.
+Proof.
+  wp_start as "@". wp_auto.
+  wp_apply wp_alloc as "* Ha".
+  wp_apply (AuditArg.wp_enc (AuditArg.mk' _) with "[$Ha]") as "* (Hsl_b&_&_&%Hwish)".
+  { iDestruct own_slice_nil as "$".
+    iDestruct own_slice_cap_nil as "$". }
+  simpl in *.
+  wp_apply wp_alloc as "* Hreply".
+  wp_apply (wp_Audit_cli_call (Q_read_idx (uint.nat prevEpoch))
+    with "[$Hsl_b $Hreply]") as "* @".
+  { iFrame "#".
+    rewrite /server.is_rpc_cli.
+    case_match; try done.
+    iNamed "His_args".
+    by iApply op_read_idx. }
+  wp_if_destruct.
+  { rewrite ktcore.rw_BlameUnknown.
+    iApply "HΦ".
+    iSplit; [|by case_decide].
+    iPureIntro. apply ktcore.blame_unknown. }
+  iNamed "Herr_net".
+  iPersist "Hsl_reply".
+  wp_apply (AuditReply.wp_dec with "[$Hsl_reply]") as "* Hgenie".
+  wp_if_destruct.
+  { rewrite ktcore.rw_BlameServFull.
+    iApply "HΦ".
+    iSplit; [|by case_decide].
+    iApply ktcore.blame_one.
+    iIntros (?).
+    case_match; try done.
+    iNamed "Hgood".
+    iApply "Hgenie".
+    naive_solver. }
+  iDestruct "Hgenie" as (??) "(#Hreply&_&%His_dec)".
+  destruct obj. iNamed "Hreply".
+  wp_auto. simpl.
+  wp_if_destruct.
+  { rewrite ktcore.rw_BlameServFull.
+    iApply "HΦ".
+    iSplit; try done.
+    iApply ktcore.blame_one.
+    iIntros (?).
+    case_match; try done.
+    iNamed "Hgood".
+    opose proof (AuditReply.wish_det _ _ _ _ His_dec His_reply) as [? _].
+    simplify_eq/=.
+    iDestruct "Hgood" as "[@|@]".
+    - iApply "Hgenie". naive_solver.
+    - opose proof (AuditArg.wish_det _ _ _ _ Hwish Hdec) as [? _].
+      simplify_eq/=.
+      iDestruct "HQ" as "[#Hnew_digs %]".
+      iDestruct "Herr" as %?.
+      lia. }
+
+  rewrite /ktcore.BlameNone ktcore.rw_BlameNone.
+  iApply "HΦ".
+  iSplit.
+  { iPureIntro. apply ktcore.blame_none. }
+  case_decide; try done.
+  iFrame "#".
+  case_match; try done.
+  iNamed "Hgood".
+  opose proof (AuditReply.wish_det _ _ _ _ His_dec His_reply) as [? _].
+  simplify_eq/=.
+  iDestruct "Hgood" as "[@|@]"; try done.
+  opose proof (AuditArg.wish_det _ _ _ _ Hwish Hdec) as [? _].
+  simplify_eq/=.
+  iDestruct "HQ" as "[#Hnew_digs %]".
+  iNamed "Herr".
+
+  iClear "His_args".
+  iApply big_sepL_intro.
+  iModIntro. iIntros (?? Hlook_proofs) "!> * @ % %Heq_sig_pk".
+  rewrite /wish_getNextLink /history.align_serv.
+  destruct adtrσ, σ. simplify_eq/=.
+  iDestruct (big_sepL_lookup with "His_upds") as "{His_upds} @"; [done|].
+  iDestruct (big_sepL_lookup with "His_sigs") as "{His_sigs} @"; [done|].
+  apply lookup_lt_Some in Hlook_proofs.
+  iDestruct (mono_list_lb_valid with "Hnew_digs His_digs") as %[[? Hpref]|[new_digs ?]].
+  { apply (f_equal length) in Hpref.
+    autorewrite with len in *. word. }
+  simplify_eq/=.
+  autorewrite with len in *.
+  iDestruct (mono_list_lb_own_le (digs ++ [dig1]) with "Hnew_digs")
+    as "{Hnew_digs His_digs} Hlb".
+  { apply prefix_snoc.
+    { by apply prefix_app_r. }
+    rewrite -Hlook1. f_equal. word. }
+
+  rewrite Heq_sig_pk.
+  iFrame "#".
+  repeat iSplit; try done; try iPureIntro.
+  - word.
+  - rewrite lookup_app_l in Hlook0; [|word].
+    replace (_ + _)%nat with (pred $ length digs) in Hlook0 by word.
+    rewrite -last_lookup in Hlook0.
+    rewrite Hlook0.
+    naive_solver.
+  - exact_eq His_link; [|done|word].
+    erewrite take_S_r.
+    2: { by erewrite <-Hlook1. }
+    rewrite take_app_length'; [done|].
+    len.
+Qed.
+
+End proof.
+End auditor.
